dimsum/spec.v
@@ -467,7 +467,7 @@ Proof.
   rewrite /equiv/spec_equiv !spec_to_itree_bind Heq1. by setoid_rewrite Heq2.
 Qed.
 
-Lemma spec_bind_bind {EV S R T U} (s : spec EV S R) (k : R → spec EV S U) (h : U → spec EV S T) :
+Lemma bind_bind {EV S R T U} (s : spec EV S R) (k : R → spec EV S U) (h : U → spec EV S T) :
   Spec.bind (Spec.bind s k) h ≡ Spec.bind s (fun r => Spec.bind (k r) h).
 Proof.
   rewrite /equiv/spec_equiv !spec_to_itree_bind bind_bind.
